mettail-rho-runtime/src/lib.rs
@@ -66,6 +66,7 @@ pub use run::{
 pub use run::{
     run_normalized_par_for_oracle, run_normalized_par_for_oracle_and_read_bools,
     run_normalized_par_for_oracle_and_read_ints,
+    run_normalized_par_for_oracle_and_read_string_channels,
     run_normalized_par_for_oracle_and_read_string_tuples,
     run_normalized_par_for_oracle_and_read_strings, run_rholang_source_for_oracle,
     run_rholang_source_for_oracle_and_read_bools, run_rholang_source_for_oracle_and_read_ints,
